arm/Asmgenproof.v
@@ -451,7 +451,7 @@ Lemma exec_straight_steps:
    exists rs2,
        exec_straight tge tf c rs1 m1' k rs2 m2'
     /\ agree ms2 sp rs2
-    /\ (r10_is_parent ep i = true -> rs2#IR10 = parent_sp s)) ->
+    /\ (it1_is_parent ep i = true -> rs2#IR10 = parent_sp s)) ->
   exists st',
   plus step tge (State rs1 m1') E0 st' /\
   match_states (Mach.State s fb sp c ms2 m2) st'.
@@ -470,7 +470,7 @@ Lemma exec_straight_steps_goto:
   Genv.find_funct_ptr ge fb = Some (Internal f) ->
   Mach.find_label lbl f.(Mach.fn_code) = Some c' ->
   transl_code_at_pc ge (rs1 PC) fb f (i :: c) ep tf tc ->
-  r10_is_parent ep i = false ->
+  it1_is_parent ep i = false ->
   (forall k c (TR: transl_instr f i ep k = OK c),
    exists jmp, exists k', exists rs2,
        exec_straight tge tf c rs1 m1' (jmp :: k') rs2 m2'
